src/Lean.v
@@ -1,4 +1,5 @@
-From Stdlib Require ZArith NArith Lia ZifyBool Uint63.
+From Stdlib Require BinInt BinNat Nnat Znat Lia ZifyBool.
+From Corelib Require Uint63Axioms.
 Declare ML Module "coq-lean-import.plugin".
 
 Set Universe Polymorphism.
@@ -21,6 +22,10 @@ Inductive eq_inst1@{|} {α:SProp} (a:α) : α -> SProp
   := eq_refl_inst1 : eq_inst1 a a.
 
 Register eq_inst1 as lean.Eq_inst1.
+
+Inductive Bool := Bool_false | Bool_true.
+
+Register Bool as lean.Bool.
 
 (* Inductive List@{u Lean.u+1.0} (α : Type@{Lean.u+1.0}) : Type@{Lean.u+1.0} :=
     List_nil : List@{u Lean.u+1.0} α
@@ -91,6 +96,7 @@ End Quot.
 Inductive Nat := Nat_zero : Nat | Nat_succ : Nat -> Nat.
 
 Register Nat as lean.Nat.
+Register Nat as kernel.ind_peano_nat.
 
 Fixpoint double (n : Nat) : Nat :=
   match n with
@@ -99,6 +105,7 @@ Fixpoint double (n : Nat) : Nat :=
   end.
 
 Register double as lean.Nat_double.
+Register double as kernel.peano_nat_double.
 
 Declare Scope Nat_scope.
 Delimit Scope Nat_scope with Nat.
@@ -129,9 +136,15 @@ Record And@{} (a a0 : SProp) : SProp := And_intro
 Register And as lean.And.
 
 Inductive sEmpty : SProp := .
+Register sEmpty as lean.False.
+
+Inductive Decidable (p : SProp) : Type :=
+| Decidable_isFalse : (p -> sEmpty) -> Decidable p
+| Decidable_isTrue : p -> Decidable p.
+Register Decidable as lean.Decidable.
 
 Section nat_notation.
-  Import ZifyClasses ZArith NArith.
+  Import ZifyClasses BinInt BinNat Nnat Znat.
   Fixpoint nat_of_Nat (n : Nat) : nat :=
     match n with
     | Nat_zero => 0
@@ -237,43 +250,149 @@ Number Notation Nat Nat_of_num_uint Nat_to_num_uint (abstract after 5000) : Nat_
 (* Tell the kernel to unfold these wrappers early, to speed things up *)
 #[global] Strategy -10000 [Nat_of_num_uint Nat_to_num_uint].
 
+Fixpoint Nat_add n m :=
+  match m with
+  | 0 => n
+  | Nat_succ p => Nat_succ (Nat_add n p)
+  end.
+
+Fixpoint Nat_mul n m :=
+  match m with
+  | 0 => 0
+  | Nat_succ p => Nat_add (Nat_mul n p) n
+  end.
+
+Fixpoint Nat_pow n m :=
+  match m with
+    | 0 => 1
+    | Nat_succ m => Nat_mul (Nat_pow n m) n
+  end.
+
+Definition Nat_pred n :=
+  match n with
+  | Nat_zero => Nat_zero
+  | Nat_succ n => n
+  end.
+
+Fixpoint Nat_sub n m :=
+  match m with
+  | Nat_zero => n
+  | Nat_succ m => Nat_pred (Nat_sub n m)
+  end.
+
+Fixpoint Nat_beq n m :=
+  match n, m with
+  | Nat_zero, Nat_zero => Bool_true
+  | Nat_succ n, Nat_succ m => Nat_beq n m
+  | _, _ => Bool_false
+  end.
+
+Fixpoint Nat_ble n m :=
+  match n, m with
+  | Nat_zero, _ => Bool_true
+  | Nat_succ _, Nat_zero => Bool_false
+  | Nat_succ n, Nat_succ m => Nat_ble n m
+  end.
+
+Definition Nat_blt n m := Nat_ble (Nat_succ n) m.
+
+Lemma Nat_beq_refl (n : Nat) : Logic.eq (Nat_beq n n) Bool_true.
+Proof.
+  induction n as [|n IH]; cbn [Nat_beq]; assumption || reflexivity.
+Qed.
+
+Lemma Nat_beq_true_eq (n m : Nat) :
+  Logic.eq (Nat_beq n m) Bool_true -> eq n m.
+Proof.
+  revert m.
+  induction n as [|n IH]; intros [|m] H; cbn [Nat_beq] in H.
+  - exact (eq_refl Nat_zero).
+  - discriminate H.
+  - discriminate H.
+  - destruct (IH m H). constructor.
+Qed.
+
+Lemma Nat_beq_false_ne (n m : Nat) :
+  Logic.eq (Nat_beq n m) Bool_false -> eq n m -> sEmpty.
+Proof.
+  intros H E.
+  destruct E.
+  rewrite Nat_beq_refl in H.
+  discriminate H.
+Qed.
+
+Definition Nat_decEq (n m : Nat) : Decidable (eq n m).
+Proof.
+  destruct (Nat_beq n m) eqn:H.
+  - exact (Decidable_isFalse _ (Nat_beq_false_ne n m H)).
+  - exact (Decidable_isTrue _ (Nat_beq_true_eq n m H)).
+Defined.
+
+Register Nat_add as lean.Nat_add.
+Register Nat_add as kernel.peano_nat_add.
+Register Nat_mul as lean.Nat_mul.
+Register Nat_mul as kernel.peano_nat_mul.
+Register Nat_pow as lean.Nat_pow.
+Register Nat_pow as kernel.peano_nat_pow.
+Register Nat_pred as lean.Nat_pred.
+Register Nat_sub as lean.Nat_sub.
+Register Nat_sub as kernel.peano_nat_sub.
+Register Nat_beq as lean.Nat_beq.
+Register Nat_beq as kernel.peano_nat_beq.
+Register Nat_ble as lean.Nat_ble.
+Register Nat_ble as kernel.peano_nat_ble.
+Register Nat_blt as lean.Nat_blt.
+Register Nat_decEq as lean.Nat_decEq.
+
+Import BinNat.
+
+
+(* Decode binary literals without an intermediate unary [nat]. *)
+Fixpoint CompactPos (p : positive) : Nat :=
+  match p with
+  | xH => Nat_succ Nat_zero
+  | xO p => double (CompactPos p)
+  | xI p => Nat_succ (double (CompactPos p))
+  end.
+
+Definition CompactNat (n : N) : Nat :=
+  match n with
+  | N0 => Nat_zero
+  | Npos p => CompactPos p
+  end.
+
+Register CompactNat as lean.Nat_of_N.eager.
+Register CompactNat as lean.Nat_of_N.
+Register CompactNat as kernel.peano_nat_of_N.
+
 #[local] Set Warnings "-abstract-large-number".
-Definition UInt32_size : Nat := 0x100000000%Nat.
+Definition UInt32_size : Nat :=
+  Nat_pow (Nat_succ (Nat_succ Nat_zero))
+    (Nat_succ (Nat_succ (Nat_succ (Nat_succ (Nat_succ (Nat_succ
+      (Nat_succ (Nat_succ (Nat_succ (Nat_succ (Nat_succ (Nat_succ
+      (Nat_succ (Nat_succ (Nat_succ (Nat_succ (Nat_succ (Nat_succ
+      (Nat_succ (Nat_succ (Nat_succ (Nat_succ (Nat_succ (Nat_succ
+      (Nat_succ (Nat_succ (Nat_succ (Nat_succ (Nat_succ (Nat_succ
+      (Nat_succ (Nat_succ Nat_zero)))))))))))))))))))))))))))))))).
 Register UInt32_size as lean.UInt32_size.
 
 Record Fin@{} (n : Nat) := Fin_mk { val : Nat; isLt : (val < n)%Nat }.
 Register Fin as lean.Fin.
 
-(* [UInt32] uses the [BitVec 32] representation from Lean 4.17 onward. *)
-
-Fixpoint Nat_add (n m : Nat) : Nat :=
-  match n with
-  | Nat_zero => m
-  | Nat_succ n => Nat_succ (Nat_add n m)
-  end.
-
-Fixpoint Nat_mul (n m : Nat) : Nat :=
-  match n with
-  | Nat_zero => Nat_zero
-  | Nat_succ n => Nat_add m (Nat_mul n m)
-  end.
-
-Fixpoint Nat_pow (b e : Nat) : Nat :=
-  match e with
-  | Nat_zero => Nat_succ Nat_zero
-  | Nat_succ e => Nat_mul b (Nat_pow b e)
-  end.
-Register Nat_pow as lean.Nat_pow.
-
-Record BitVec@{} (w : Nat) : Type := BitVec_mk { toFin : Fin (Nat_pow 2 w) }.
+Record BitVec@{} (w : Nat) := BitVec_mk { toFin : Fin (Nat_pow 2 w) }.
 Register BitVec as lean.BitVec.
 
 Record UInt32@{} := UInt32_mk { toBitVec : BitVec 32 }.
 Register UInt32 as lean.UInt32.
+Register toBitVec as lean.toBitVec.
+
+Definition UInt32_toNat (n : UInt32) : Nat :=
+  n.(toBitVec).(toFin _).(val _).
+Register UInt32_toNat as lean.UInt32_toNat.
 
 
 Section strings.
-  Import ZArith NArith Lia Zify ZifyBool.
+  Import BinInt BinNat Nnat Znat Lia Zify ZifyBool.
   Variant InvalidUInt32 (n : N) : Set := invalid_uint32.
   Variant InvalidChar (n : N) : Set := invalid_char.
   #[local] Set Warnings "-abstract-large-number".
@@ -317,7 +436,11 @@ Section strings.
   #[local] Open Scope Nat_scope.
 
   Definition Nat_isValidChar (n : Nat) : SProp
-    := n < 0xd800 \/ (0xdfff < n /\ n < 0x110000).
+    := n < CompactNat 0xd800%N \/
+       (CompactNat 0xdfff%N < n /\ n < CompactNat 0x110000%N).
+
+  Definition UInt32_isValidChar (n : UInt32) : SProp :=
+    Nat_isValidChar n.(toBitVec).(toFin _).(val _).
 
   Record Char@{} := Char_mk
   { val1 : UInt32; valid : Nat_isValidChar val1.(toBitVec).(toFin _).(val _) }.
@@ -325,71 +448,105 @@ Section strings.
   Definition check_N_isValidChar (n : N) : bool
     := ((n <? 0xd800) || ((0xdfff <? n) && (n <? 0x110000)))%N%bool.
 
-  Definition Fin_mk_N (n : N) (val : N) (isLt : (val <? n)%N = true) : Fin (Nat_of_N n)
-    := Fin_mk (Nat_of_N n) (Nat_of_N val) (Nat_lt_to_N val n isLt).
-
-  Lemma Fin_eq_rec_r_val (n m : Nat) (x : Fin n) (H : m = n)
-    : Lean.val m (eq_rec_r (fun n => Fin n) x H) = Lean.val n x.
-  Proof. destruct H; reflexivity. Qed.
-
-  Lemma nat_of_Nat_add (n m : Nat)
-    : nat_of_Nat (Nat_add n m) = (nat_of_Nat n + nat_of_Nat m)%nat.
-  Proof. induction n; cbn; rewrite ?IHn; reflexivity. Qed.
-
-  Lemma N_of_Nat_add (n m : Nat)
-    : N_of_Nat (Nat_add n m) = (N_of_Nat n + N_of_Nat m)%N.
-  Proof. cbv [N_of_Nat]; rewrite nat_of_Nat_add, Nat2N.inj_add; reflexivity. Qed.
-
-  Lemma N_of_Nat_succ (n : Nat)
-    : N_of_Nat (Nat_succ n) = N.succ (N_of_Nat n).
-  Proof. unfold N_of_Nat; cbn [nat_of_Nat]; rewrite Nat2N.inj_succ; reflexivity. Qed.
-
-  Lemma N_of_Nat_mul (n m : Nat)
-    : N_of_Nat (Nat_mul n m) = (N_of_Nat n * N_of_Nat m)%N.
+  Lemma Nat_nat_add n m : Nat_of_nat (n + m) = Nat_add (Nat_of_nat n) (Nat_of_nat m).
   Proof.
-    induction n; cbn [Nat_mul]; [ reflexivity | ].
-    rewrite N_of_Nat_add, IHn.
-    rewrite N_of_Nat_succ, N.mul_succ_l, N.add_comm; reflexivity.
+    rewrite Nat.add_comm.
+    induction m.
+    - reflexivity.
+    - simpl. now f_equal.
   Qed.
 
-  Lemma N_of_Nat_pow (b e : Nat)
-    : N_of_Nat (Nat_pow b e) = (N_of_Nat b ^ N_of_Nat e)%N.
+  Lemma Nat_nat_mul n m : Nat_of_nat (n * m) = Nat_mul (Nat_of_nat n) (Nat_of_nat m).
   Proof.
-    induction e; cbn [Nat_pow]; [ reflexivity | ].
-    rewrite N_of_Nat_mul, IHe, N_of_Nat_succ, N.pow_succ_r'; reflexivity.
+    rewrite Nat.mul_comm.
+    induction m; simpl.
+    - reflexivity.
+    - rewrite Nat.add_comm, Nat_nat_add. now f_equal.
   Qed.
 
-  Lemma N_of_Nat_inj (n m : Nat) : N_of_Nat n = N_of_Nat m -> n = m.
+  Lemma Nat_nat_pow n m : Nat_of_nat (n ^ m) = Nat_pow (Nat_of_nat n) (Nat_of_nat m).
   Proof.
-    cbv [N_of_Nat].
-    intro H; apply (f_equal N.to_nat) in H; rewrite !Nat2N.id in H.
-    apply (f_equal Nat_of_nat) in H; rewrite !Nat2natid in H; exact H.
+    induction m; simpl.
+    - reflexivity.
+    - rewrite Nat.mul_comm, Nat_nat_mul. now f_equal.
   Qed.
 
-  Lemma N_of_Nat_of_N (n : N) : N_of_Nat (Nat_of_N n) = n.
-  Proof. unfold N_of_Nat, Nat_of_N; rewrite nat2Natid, N2Nat.id; reflexivity. Qed.
-
-  Lemma Nat_pow_2_32 : Nat_pow 2 32 = Nat_of_N 0x100000000.
+  Lemma Nat_pow_comm (n : N) : Nat_of_N (2 ^ n) = Nat_pow 2 (Nat_of_N n).
   Proof.
-    apply N_of_Nat_inj; rewrite N_of_Nat_pow, N_of_Nat_of_N.
-    vm_compute; reflexivity.
+    unfold Nat_of_N. rewrite N2Nat.inj_pow.
+    eapply Nat_nat_pow.
   Qed.
 
-  Definition UInt32_mk_N (val : N) (isLt : (val <? 0x100000000)%N = true) : UInt32.
+  Lemma double_Nat_of_nat (n : nat) :
+    double (Nat_of_nat n) = Nat_of_nat (n + n).
   Proof.
-    refine (UInt32_mk (BitVec_mk 32 _)).
-    rewrite Nat_pow_2_32.
-    exact (Fin_mk_N 0x100000000 val isLt).
-  Defined.
+    induction n as [|n IHn].
+    - reflexivity.
+    - cbn [double Nat_of_nat Nat.add].
+      rewrite Nat.add_succ_r, IHn.
+      reflexivity.
+  Qed.
 
-  Lemma UInt32_mk_N_val (val : N) (isLt : (val <? 0x100000000)%N = true)
-    : (UInt32_mk_N val isLt).(toBitVec).(toFin _).(Lean.val _) = Nat_of_N val.
-  Proof. unfold UInt32_mk_N; apply Fin_eq_rec_r_val. Qed.
+  Lemma CompactPos_eq_Nat_of_nat (p : positive) :
+    CompactPos p = Nat_of_nat (Pos.to_nat p).
+  Proof.
+    induction p as [p IHp | p IHp |].
+    - rewrite Pos2Nat.inj_xI.
+      replace (2 * Pos.to_nat p)%nat with
+        (Pos.to_nat p + Pos.to_nat p)%nat by lia.
+      cbn [CompactPos Nat_of_nat].
+      now rewrite IHp, double_Nat_of_nat.
+    - rewrite Pos2Nat.inj_xO.
+      replace (2 * Pos.to_nat p)%nat with
+        (Pos.to_nat p + Pos.to_nat p)%nat by lia.
+      cbn [CompactPos].
+      now rewrite IHp, double_Nat_of_nat.
+    - reflexivity.
+  Qed.
+
+  Lemma CompactNat_eq_Nat_of_N (n : N) : CompactNat n = Nat_of_N n.
+  Proof.
+    destruct n as [|p].
+    - reflexivity.
+    - apply CompactPos_eq_Nat_of_nat.
+  Qed.
+
+  Lemma CompactNat_lt_to_N (n m : N) :
+    (n <? m)%N = true -> CompactNat n < CompactNat m.
+  Proof.
+    rewrite !CompactNat_eq_Nat_of_N.
+    apply Nat_lt_to_N.
+  Qed.
+
+  Lemma CompactNat_pow_comm (n : N) :
+    CompactNat (2 ^ n) = Nat_pow 2 (CompactNat n).
+  Proof.
+    rewrite !CompactNat_eq_Nat_of_N.
+    apply Nat_pow_comm.
+  Qed.
+
+  Lemma Nat_lt_to_N_pow (n : N) (m : N) :
+    (n <? 2 ^ m)%N = true -> Nat_of_N n < Nat_pow 2 (CompactNat m).
+  Proof.
+    rewrite <- CompactNat_pow_comm, CompactNat_eq_Nat_of_N.
+    apply Nat_lt_to_N.
+  Qed.
+
+  Definition Fin_mk_N_pow (n : N) (val : N)
+      (isLt : (val <? 2 ^ n)%N = true) :
+      Fin (Nat_pow 2 (CompactNat n)) :=
+    Fin_mk (Nat_pow 2 (CompactNat n)) (Nat_of_N val)
+      (Nat_lt_to_N_pow val n isLt).
+
+  Definition UInt32_mk_N (val : N) (isLt : (val <? 0x100000000)%N = true) : UInt32
+    := UInt32_mk (BitVec_mk 32 (Fin_mk_N_pow 32 val isLt)).
 
   Lemma Nat_isValidChar_mk_N (n : N) (isLt : check_N_isValidChar n = true)
     : Nat_isValidChar (Nat_of_N n).
   Proof.
-    cbv [Nat_isValidChar Nat_of_num_uint check_N_isValidChar] in *.
+    unfold Nat_isValidChar.
+    rewrite !CompactNat_eq_Nat_of_N.
+    cbv [Nat_of_num_uint check_N_isValidChar] in *.
     pose proof (Nat_lt_to_N n 0xd800) as H1.
     pose proof (Nat_lt_to_N 0xdfff n) as H2.
     pose proof (Nat_lt_to_N n 0x110000) as H3.
@@ -410,12 +567,9 @@ Section strings.
     all: vm_compute; congruence.
   Qed.
 
-  Definition Char_mk_N (val : N) (isLt : ((val <? 0x100000000)%N && check_N_isValidChar val)%bool = true) : Char.
-  Proof.
-    refine (Char_mk (UInt32_mk_N val (proj1 (andb_prop _ _ isLt))) _).
-    rewrite UInt32_mk_N_val.
-    exact (Nat_isValidChar_mk_N val (proj2 (andb_prop _ _ isLt))).
-  Defined.
+  Definition Char_mk_N (val : N) (isLt : ((val <? 0x100000000)%N && check_N_isValidChar val)%bool = true) : Char
+    := Char_mk (UInt32_mk_N val (proj1 (andb_prop _ _ isLt)))
+         (Nat_isValidChar_mk_N val (proj2 (andb_prop _ _ isLt))).
 
   Definition reflective_Char_mk (val : N)
     : if ((val <? 0x100000000)%N && check_N_isValidChar val)%bool
@@ -427,8 +581,9 @@ Section strings.
        | false => fun _ => invalid_char val
        end Logic.eq_refl.
 
-  Definition reflective_Char_mk_prim (val : Uint63.int)
-    := reflective_Char_mk (Z.to_N (Uint63.to_Z val)).
+  Definition reflective_Char_mk_prim (val : PrimInt63.int)
+    := reflective_Char_mk (Z.to_N (Uint63Axioms.to_Z val)).
+
 
   (* Definition reflective_UInt32_mk (val : N) : if (val <? 0x100000000)%N
                                               then UInt32
@@ -439,8 +594,8 @@ Section strings.
        | false => fun _ => invalid_uint32 val
        end Logic.eq_refl.
 
-  Definition reflective_UInt32_mk_prim (val : Uint63.int)
-    := reflective_UInt32_mk (Z.to_N (Uint63.to_Z val)).
+  Definition reflective_UInt32_mk_prim (val : PrimInt63.int)
+    := reflective_UInt32_mk (Z.to_N (Uint63Axioms.to_Z val)).
 
 
   Definition check_isValidChar (n : Nat) : bool
@@ -478,5 +633,6 @@ Section strings.
 End strings.
 
 Register Nat_isValidChar as lean.Nat_isValidChar.
+Register UInt32_isValidChar as lean.UInt32_isValidChar.
 Register Char as lean.Char.
 Register reflective_Char_mk_prim as lean.Char.mk.reflective_prim.
