tests/compact_nat.v
@@ -1,0 +1,6 @@
+From Stdlib Require Import NArith.BinNat.
+From LeanImport Require Import Lean.
+
+Example compact_nat_exposes_one_constructor :
+  eq (CompactNat 1000000%N) (Nat_succ (CompactNat 999999%N)).
+Proof. reflexivity. Qed.
