tests/nat_boolean_source_reload.v
@@ -1,0 +1,2 @@
+Require Import nat_boolean_source.
+Check Nat_beq_eq_def.
